# baseURI: https://w3id.org/nen2660/skos/term
# imports: http://qudt.org/2.1/schema/qudt
# imports: http://qudt.org/2.1/vocab/quantitykind
# imports: http://qudt.org/2.1/vocab/unit
# imports: http://www.w3.org/2004/02/skos/core
# imports: http://www.w3.org/2006/time
# imports: http://www.w3.org/ns/shacl
# prefix: nen2660-term

@prefix nen2660-term: <https://w3id.org/nen2660/term#> .
@prefix owl: <http://www.w3.org/2002/07/owl#> .
@prefix quantitykind: <http://qudt.org/vocab/quantitykind/> .
@prefix qudt: <http://qudt.org/schema/qudt/> .
@prefix rdf: <http://www.w3.org/1999/02/22-rdf-syntax-ns#> .
@prefix rdfs: <http://www.w3.org/2000/01/rdf-schema#> .
@prefix sh: <http://www.w3.org/ns/shacl#> .
@prefix skos: <http://www.w3.org/2004/02/skos/core#> .
@prefix time: <http://www.w3.org/2006/time#> .
@prefix unit: <http://qudt.org/vocab/unit/> .
@prefix xsd: <http://www.w3.org/2001/XMLSchema#> .

<https://w3id.org/nen2660/skos/term>
  a skos:ConceptScheme ;
  owl:imports <http://qudt.org/2.1/schema/qudt> ;
  owl:imports <http://qudt.org/2.1/vocab/quantitykind> ;
  owl:imports <http://qudt.org/2.1/vocab/unit> ;
  owl:imports <http://www.w3.org/2004/02/skos/core> ;
  owl:imports <http://www.w3.org/2006/time> ;
  owl:imports <http://www.w3.org/ns/shacl> ;
  skos:hasTopConcept nen2660-term:TopConcept ;
.
nen2660-term:AbstractConcept
  a skos:Concept ;
  skos:broader nen2660-term:TopConcept ;
  skos:definition "Concept dat een manifestatie en een afbakening vormt in een abstracte ruimte. Een abstract concept heeft geen levenscyclus"@nl ;
  skos:definition "Concept that forms a manifestation and demarcation in an abstract space. An abstract concept has no life cycle"@en ;
  skos:prefLabel "Abstract concept"@en ;
  skos:prefLabel "Abstract concept"@nl ;
.
nen2660-term:Activity
  a skos:Concept ;
  skos:broader nen2660-term:Entity ;
  skos:definition "Entiteit die plaatsvindt of kan plaatsvinden in een concrete ruimte-tijd. Een activiteit transformeert objecten, en wordt uitgevoerd door een object"@nl ;
  skos:definition "Entity that takes place or can take place in a concrete space-time. An activity transforms objects, and is executed by an object"@en ;
  skos:prefLabel "Activity"@en ;
  skos:prefLabel "Activiteit"@nl ;
.
nen2660-term:AggregationStateType
  a skos:Concept ;
  skos:broader nen2660-term:EnumerationType ;
  skos:definition "Een van de vier fundamentele toestanden van materie zijnde een vaste stof, vloeistof, gas of plasma"@nl ;
  skos:definition "One of the four fundamental states of matter being a solid, liquid, gas or plasma"@en ;
  skos:prefLabel "Aggregatietoestandtype"@nl ;
  skos:prefLabel "Aggregation state type"@en ;
.
nen2660-term:AmountOfBulkMatter
  a skos:Concept ;
  skos:broader nen2660-term:RealObject ;
  skos:definition "A real object that consists of a continuous amount of non-rigid matter, held together primarily by external forces (gravity or confinement)"@en ;
  skos:definition "Een reëel object dat bestaat uit een aaneengesloten hoeveelheid niet-vormvaste materie, primair bijeengehouden door externe krachten (zwaartekracht of opsluiting)"@nl ;
  skos:prefLabel "Amount of bulk matter"@en ;
  skos:prefLabel "Hoeveelheid bulkmaterie"@nl ;
.
nen2660-term:ChemicalCompound
  a skos:Concept ;
  skos:broader nen2660-term:PureSubstance ;
  skos:definition "Pure substance consisting of two or more chemical elements that have a chemical bond with each other. In a chemical compound, the elements occur in a fixed ratio. A compound can be broken down into simpler substances by means of chemical reactions"@en ;
  skos:definition "Zuivere stof bestaande uit twee of meer chemische elementen die een chemische binding met elkaar hebben. In een chemische verbinding komen de elementen in een vaste verhouding voor. Een verbinding kan worden ontleed in eenvoudigere stoffen door middel van chemische reacties"@nl ;
  skos:prefLabel "Chemical compound"@en ;
  skos:prefLabel "Chemische verbinding"@nl ;
.
nen2660-term:ChemicalElement
  a skos:Concept ;
  skos:broader nen2660-term:PureSubstance ;
  skos:definition "Pure substance that is made up of atoms with the same atomic number. A chemical element cannot be decomposed through chemical reactions"@en ;
  skos:definition "Zuivere stof die is opgebouwd uit atomen met hetzelfde atoomnummer. Een chemisch element kan niet worden ontleed door middel van chemische reacties"@nl ;
  skos:prefLabel "Chemical element"@en ;
  skos:prefLabel "Chemisch element"@nl ;
.
nen2660-term:ConceptType
  a skos:Concept ;
  skos:broader nen2660-term:Type ;
  skos:definition "A meta-concept having concepts as instances that can have attributes or relations"@en ;
  skos:definition "Een meta-concept met concepten als instanties die attributen of relaties kunnen hebben"@nl ;
  skos:prefLabel "Concept type"@en ;
  skos:prefLabel "Concept type"@nl ;
.
nen2660-term:ConcreteConcept
  a skos:Concept ;
  skos:broader nen2660-term:TopConcept ;
  skos:definition "Concept dat een manifestatie en een afbakening vormt in een concrete ruimte-tijd. Een concreet concept heeft een levenscyclus"@nl ;
  skos:definition "Concept that forms a manifestation and a demarcation in a concrete space-time. A concrete concept has a life cycle"@en ;
  skos:prefLabel "Concreet concept"@nl ;
  skos:prefLabel "Concrete concept"@en ;
.
nen2660-term:Connection
  a skos:Concept ;
  skos:broader nen2660-term:PhysicalObject ;
  skos:definition "A physical object (real object or spatial area) that connects two other physical objects and over which interaction takes place, namely the transfer of matter, energy, information or forces"@en ;
  skos:definition "Een fysiek object (reëel object of ruimtelijk gebied) dat twee andere fysieke objecten verbindt en waarover interactie plaatsvindt namelijk de overdracht van materie, energie, informatie of krachten"@nl ;
  skos:prefLabel "Connection"@en ;
  skos:prefLabel "Verbinding"@nl ;
.
nen2660-term:DiscreteObject
  a skos:Concept ;
  skos:broader nen2660-term:RealObject ;
  skos:definition "A real object consisting of a contiguous amount of form-retaining matter, held together primarily by internal forces (gravity or electromagnetic force)"@en ;
  skos:definition "Een reëel object dat bestaat uit een aaneengesloten hoeveelheid vormvaste materie, primair bijeengehouden door interne krachten (zwaartekracht of elektromagnetische kracht)"@nl ;
  skos:prefLabel "Discreet object"@nl ;
  skos:prefLabel "Discrete object"@en ;
.
nen2660-term:EnergyFlow
  a skos:Concept ;
  skos:broader nen2660-term:TransferType ;
  skos:definition "De beweging van een hoeveelheid energie (als capaciteit om arbeid te verrichten)"@nl ;
  skos:definition "The movement of an amount of energy (as capacity to do work)"@en ;
  skos:prefLabel "Energie stroom"@nl ;
  skos:prefLabel "Energy flow"@en ;
.
nen2660-term:Entity
  a skos:Concept ;
  skos:broader nen2660-term:ConcreteConcept ;
  skos:definition "Concept dat een manifestatie en een afbakening vormt in een concrete ruimte-tijd, en dat op ieder moment in de tijd een bepaalde toestand heeft. Een entiteit heeft een unieke identiteit die constant blijft gedurende de levenscyclus. De levenscyclus van een entiteit is opgebouwd uit de reeks van toestanden van die entiteit, die elkaar in de tijd opvolgen. Een entiteit is een object of een activiteit. Een object bestaat, een activiteit vindt plaats"@nl ;
  skos:definition "Concept that forms a manifestation and a demarcation in a concrete space-time, and which has a certain state at any moment in time. An entity has a unique identity that remains constant throughout its life cycle. The life cycle of an entity is made up of the sequence of states of that entity, which follow each other in time. An entity is an object or an activity. An object exists, an activity takes place"@en ;
  skos:prefLabel "Entiteit"@nl ;
  skos:prefLabel "Entity"@en ;
.
nen2660-term:EnumerationType
  a skos:Concept ;
  skos:broader nen2660-term:Type ;
  skos:definition "A meta-concept having concepts as instances having no further attributes or relations (annotations only)"@en ;
  skos:definition "Een meta-concept met concepten als instanties zonder verdere attributen of relaties (alleen annotaties)"@nl ;
  skos:prefLabel "Enumeratie type"@nl ;
  skos:prefLabel "Enumeration type"@en ;
.
nen2660-term:Event
  a skos:Concept ;
  skos:broader nen2660-term:ConcreteConcept ;
  skos:definition "Overgang tussen twee opeenvolgende toestanden van een entiteit (object of activiteit). Een gebeurtenis wordt getriggerd in een toestand"@nl ;
  skos:definition "Transition between two successive states of an entity (object or activity). An event is triggered in a state"@en ;
  skos:prefLabel "Event"@en ;
  skos:prefLabel "Gebeurtenis"@nl ;
.
nen2660-term:Force
  a skos:Concept ;
  skos:broader nen2660-term:TransferType ;
  skos:definition "Natuurkundige grootheid die, uitgeoefend op een lichaam, daarin een spanning of druk doet ontstaan, of die het lichaam van beweging doet veranderen, doet versnellen"@nl ;
  skos:definition "Physical quantity which, when exerted on a body, causes tension or pressure to arise therein, or which causes the body to change motion, accelerate"@en ;
  skos:prefLabel "Force"@en ;
  skos:prefLabel "Kracht"@nl ;
.
nen2660-term:FunctionalEntity
  a skos:Concept ;
  skos:broader nen2660-term:Entity ;
  skos:definition "An entity involving the external behavior where the output contributes to stakeholder objectives implemented/played by one or more technical entities"@en ;
  skos:definition "Een entiteit waarbij het gaat om het externe gedrag waarbij de uitvoer bijdraagt aan doelstellingen van belanghebbenden geïmplementeerd/gespeeld door een of meer technische entiteiten"@nl ;
  skos:prefLabel "Functional entity"@en ;
  skos:prefLabel "Functionele entiteit"@nl ;
.
nen2660-term:Gas
  a skos:Concept ;
  skos:broader nen2660-term:AggregationStateType ;
  skos:definition "Materie in een tussentoestand tussen vloeistof en plasma die alleen kan worden ingesloten als deze volledig is omgeven door een vaste stof (of in een bel van vloeistof) (of bij elkaar wordt gehouden door zwaartekracht); het kan condenseren tot een vloeistof, of kan (zelden) direct een vaste stof worden door afzetting"@nl ;
  skos:definition "Matter in an intermediate state between liquid and plasma that can be contained only if it is fully surrounded by a solid (or in a bubble of liquid) (or held together by gravitational pull); it can condense into a liquid, or can (rarely) become a solid directly by deposition"@en ;
  skos:prefLabel "Gas"@en ;
  skos:prefLabel "Gas"@nl ;
.
nen2660-term:GeometricEntity
  a skos:Concept ;
  skos:broader nen2660-term:Representation ;
  skos:definition "Benoemd concept, dat een daadwerkelijke of virtuele afbakening vormt in een concrete (fysieke, driedimensionale) ruimte, die we in de werkelijkheid ervaren"@nl ;
  skos:definition "Named concept, which forms an actual or virtual demarcation in a concrete (physical, three-dimensional) space, which we experience in reality"@en ;
  skos:prefLabel "Geometric entity"@en ;
  skos:prefLabel "Geometrische entiteit"@nl ;
.
nen2660-term:HeterogeneousMixture
  a skos:Concept ;
  skos:broader nen2660-term:Mixture ;
  skos:definition "A mixture that is separated into different regions or phases that have different compositions or properties"@en ;
  skos:definition "Een mengsel dat is opgedeeld in verschillende regio's of fasen met verschillende samenstellingen of eigenschappen"@nl ;
  skos:prefLabel "Heterogeneen mengsel"@nl ;
  skos:prefLabel "Heterogeneous mixture"@en ;
.
nen2660-term:HomogeneousMixture
  a skos:Concept ;
  skos:broader nen2660-term:Mixture ;
  skos:definition "A mixture that is uniform throughout, and has only one phase"@en ;
  skos:definition "Een mengsel dat overal uniform is en maar 1 fase heeft"@nl ;
  skos:prefLabel "Homogeen mengsel"@nl ;
  skos:prefLabel "Homogeneous mixture"@en ;
.
nen2660-term:InformationFlow
  a skos:Concept ;
  skos:broader nen2660-term:TransferType ;
  skos:definition "De beweging van informatie weergegeven in een of ander medium"@nl ;
  skos:definition "The movement of information represented in some medium"@en ;
  skos:prefLabel "Informatie stroom"@nl ;
  skos:prefLabel "Information flow"@en ;
.
nen2660-term:InformationObject
  a skos:Concept ;
  skos:broader nen2660-term:Object ;
  skos:definition "Object dat een beschrijving vormt van een ding in de werkelijkheid"@nl ;
  skos:definition "Object which describes a thing in reality"@en ;
  skos:prefLabel "Informatie object"@nl ;
  skos:prefLabel "Information object"@en ;
.
nen2660-term:Interaction
  a skos:Concept ;
  skos:broader nen2660-term:Activity ;
  skos:definition "De activiteit zijnde een combinatie van subactiviteiten uitgevoerd door fysieke objecten waartussen een overdracht van materie, informatie, energie of kracht plaatsvindt, typisch over een verbinding of raakvlak (direct of via poorten)"@nl ;
  skos:definition "The activity being a combination of sub-activities performed by physical objects between which a transfer of matter, information, energy or force takes place, typically over a connection or interface (directly or through ports)"@en ;
  skos:prefLabel "Interactie"@nl ;
  skos:prefLabel "Interaction"@en ;
.
nen2660-term:Interface
  a skos:Concept ;
  skos:broader nen2660-term:SpatialRegion ;
  skos:definition "A spatial object, typically a thin 2D physical space (but also 0D or 1D) that connects two physical objects or ports of physical objects through which a static or dynamic interaction or interaction between those elements can take place"@en ;
  skos:definition "Een ruimtelijk object, typisch een dunne 2D fysieke ruimte (maar 0D of 1D kan ook) dat de verbinding legt tussen twee fysieke objecten of poorten van fysieke objecten waarlangs een statische of dynamische wisselwerking of interactie tussen die elementen kan plaatsvinden"@nl ;
  skos:prefLabel "Interface"@en ;
  skos:prefLabel "Raakvlak"@nl ;
.
nen2660-term:Liquid
  a skos:Concept ;
  skos:broader nen2660-term:AggregationStateType ;
  skos:definition "A liquid is a nearly incompressible fluid that conforms to the shape of its container but retains a (nearly) constant volume independent of pressure"@en ;
  skos:definition "Een vloeistof is een bijna onsamendrukbare vloeistof die zich aanpast aan de vorm van de houder, maar een (bijna) constant volume behoudt, onafhankelijk van de druk"@nl ;
  skos:prefLabel "Liquid"@en ;
  skos:prefLabel "Vloeistof"@nl ;
.
nen2660-term:MaterialFlow
  a skos:Concept ;
  skos:broader nen2660-term:TransferType ;
  skos:definition "De beweging van een hoeveelheid materiaal"@nl ;
  skos:definition "The movement of an amount of material"@en ;
  skos:prefLabel "Materiaalstroom"@nl ;
  skos:prefLabel "Material flow"@en ;
.
nen2660-term:Matter
  a skos:Concept ;
  skos:altLabel "Chemical substance"@en ;
  skos:broader nen2660-term:PhysicalObject ;
  skos:definition "A pure chemical substance, chemical compound or mixture from which real objects are made"@en ;
  skos:definition "Een pure chemische stof, chemische verbinding of mengsel waaruit reële objecten zijn gemaakt"@nl ;
  skos:prefLabel "Materie"@nl ;
  skos:prefLabel "Matter"@en ;
.
nen2660-term:MatterPortion
  a skos:Concept ;
  skos:broader nen2660-term:RelationReference ;
  skos:definition "An objectified relation reference for the consists of relation"@en ;
  skos:definition "Een geobjectiveerde relatiereferentie voor de bestaat uit relatie"@nl ;
  skos:prefLabel "Materie-aandeel"@nl ;
  skos:prefLabel "Matter portion"@en ;
.
nen2660-term:Mixture
  a skos:Concept ;
  skos:broader nen2660-term:Matter ;
  skos:definition "De combinatie van twee of meer verschillende zuivere stoffen zonder dat daarbij de moleculen hun identiteit verliezen"@nl ;
  skos:definition "The combination of two or more different pure substances without the molecules losing their identity"@en ;
  skos:prefLabel "Mengsel"@nl ;
  skos:prefLabel "Mixture"@en ;
.
nen2660-term:Object
  a skos:Concept ;
  skos:broader nen2660-term:Entity ;
  skos:definition "Entiteit die bestaat of kan bestaan binnen een concrete ruimte-tijd. Een object voert een activiteit uit, en wordt getransformeerd door een activiteit"@nl ;
  skos:definition "Entity that exists or can exist within a concrete space-time. An object executes an activity, and is transformed by an activity"@en ;
  skos:prefLabel "Object"@en ;
  skos:prefLabel "Object"@nl ;
.
nen2660-term:Objectification
  a skos:Concept ;
  skos:broader nen2660-term:AbstractConcept ;
  skos:definition "An attribute (quality or quantity) or relation represented as an individual defined by a concept"@en ;
  skos:definition "Een attribuut (kwaliteit of kwantiteit) of relatie voorgesteld als een individu gedefinieerd door een concept"@nl ;
  skos:prefLabel "Objectificatie"@nl ;
  skos:prefLabel "Objectification"@en ;
.
nen2660-term:PhysicalObject
  a skos:Concept ;
  skos:broader nen2660-term:Object ;
  skos:definition "Object dat bestaat of kan bestaan binnen de fysieke 4D ruimte-tijd. Een fysiek object vormt een manifestatie en een afbakening van materie en/of energie, en is (in)direct waarneembaar door de zintuigen"@nl ;
  skos:definition "Object that exists or may exist within physical 4D space-time. A physical object forms a manifestation and a demarcation of matter and/or energy, and is (in)directly perceptible by the senses"@en ;
  skos:prefLabel "Fysiek object"@nl ;
  skos:prefLabel "Physical object"@en ;
.
nen2660-term:PlannedEntity
  a skos:Concept ;
  skos:broader nen2660-term:Entity ;
  skos:definition "An entity that does not yet exist in physical reality, but which exists in mental or conceptual reality"@en ;
  skos:definition "Een entiteit die nog niet bestaat in de fysieke werkelijkheid, maar die in de mentale of conceptuele werkelijkheid voorkomt"@nl ;
  skos:prefLabel "Geplande entiteit"@nl ;
  skos:prefLabel "Planned entity"@en ;
.
nen2660-term:Plasma
  a skos:Concept ;
  skos:broader nen2660-term:AggregationStateType ;
  skos:definition "A phase in which the particles of a gaseous substance are ionised"@en ;
  skos:definition "Een fase waarin de deeltjes van een gasvormige stof geïoniseerd zijn"@nl ;
  skos:prefLabel "Plasma"@en ;
  skos:prefLabel "Plasma"@nl ;
.
nen2660-term:Port
  a skos:Concept ;
  skos:broader nen2660-term:PhysicalObject ;
  skos:definition "A physical or logical point of interaction as part of a physical object where, through a connection or interface, an interaction can take place"@en ;
  skos:definition "Een fysiek of logisch interactiepunt als deel van een fysiek object waar, via een verbinding of raakvlak, een interactie kan plaatsvinden"@nl ;
  skos:prefLabel "Poort"@nl ;
  skos:prefLabel "Port"@en ;
.
nen2660-term:PureSubstance
  a skos:Concept ;
  skos:broader nen2660-term:Matter ;
  skos:definition "Een chemische stof die een gelijke chemische samenstelling en herkenbare uniforme en isotrope eigenschappen heeft"@nl ;
  skos:definition "Chemical matter that has an equal chemical composition and recognizable uniform and isotropic properties"@en ;
  skos:prefLabel "Pure substance"@en ;
  skos:prefLabel "Zuivere stof"@nl ;
.
nen2660-term:QualityValue
  a skos:Concept ;
  skos:broader nen2660-term:Objectification ;
  skos:definition "De objectivering van een waarde van een kwaliteit met een complexe waarde zoals een eenvoudige waarde sec gecombineerd met andere metadata of alleen een combinatie van eenvoudige waarden"@nl ;
  skos:definition "The objectification of a value of a quality having a complex value like a simple value sec combined with other metadata or just a combination of simple values"@en ;
  skos:prefLabel "Kwaliteitwaarde"@nl ;
  skos:prefLabel "Quality value"@en ;
.
nen2660-term:QuantityKind
  a skos:Concept ;
  skos:definition "Any observable property that can be measured and quantified numerically"@en ;
  skos:definition "Elke waarneembare eigenschap die numeriek kan worden gemeten en gekwantificeerd"@nl ;
  skos:prefLabel "Kwantiteitsoort"@nl ;
  skos:prefLabel "Quantity kind"@en ;
.
nen2660-term:QuantityValue
  a skos:Concept ;
  skos:broader nen2660-term:Objectification ;
  skos:definition "De objectivering van een waarde van een hoeveelheid (typisch met een grootheid en een eenheid) met een complexe waarde zoals een eenvoudige waarde sec gecombineerd met andere metadata of alleen een combinatie van eenvoudige waarden"@nl ;
  skos:definition "The objectification of a value of a quantity (typically involving a quantity kind and a unit) having a complex value like a simple value sec combined with other metadata or just a combination of simple values"@en ;
  skos:prefLabel "Kwantiteitsoort"@nl ;
  skos:prefLabel "Quantity value"@en ;
.
nen2660-term:RealObject
  a skos:Concept ;
  skos:altLabel "Amount of matter"@en ;
  skos:broader nen2660-term:PhysicalObject ;
  skos:definition "Een fysiek object (vormvast of niet-vormvast) dat in de werkelijkheid tastbaar en zichtbaar is (of kan zijn), door de mens gemaakt of natuurlijk ontstaan"@nl ;
  skos:definition "physical object (rigid or non-rigid) that is (or can be) tangible and visible in reality, man-made or naturally occurring"@en ;
  skos:prefLabel "Real object"@en ;
  skos:prefLabel "Reeel object"@nl ;
.
nen2660-term:RealizedEntity
  a skos:Concept ;
  skos:broader nen2660-term:Entity ;
  skos:definition "An entity that exists or has existed in the physical reality"@en ;
  skos:definition "Een entiteit die bestaat of heeft bestaan in de fysieke werkelijkheid"@nl ;
  skos:prefLabel "Gerealiseerde entiteit"@nl ;
  skos:prefLabel "Realized entity"@en ;
.
nen2660-term:RelationReference
  a skos:Concept ;
  skos:broader nen2660-term:Objectification ;
  skos:definition "De objectivering van een referentie voor een relatie met een complexe waarde zoals een simpele referentie sec gecombineerd met andere metadata of alleen een combinatie van simpele referenties (n-ary relaties)"@nl ;
  skos:definition "The objectification of a reference for a relation having a complex value like a simple reference sec combined with other metadata or just a combination of simple references (n-ary relation)"@en ;
  skos:prefLabel "Relatie referentie"@nl ;
  skos:prefLabel "Relation reference"@en ;
.
nen2660-term:Representation
  a skos:Concept ;
  skos:broader nen2660-term:InformationObject ;
  skos:definition "Dat wat iets anders vertegenwoordigt"@nl ;
  skos:definition "That which represents something else"@en ;
  skos:prefLabel "Representatie"@nl ;
  skos:prefLabel "Representation"@en ;
.
nen2660-term:Requirement
  a skos:Concept ;
  skos:broader nen2660-term:InformationObject ;
  skos:definition "A rule that should hold for something, defined via its attributes or relations"@en ;
  skos:definition "Een regel die ergens voor moet gelden, gedefinieerd via zijn attributen of relaties"@nl ;
  skos:prefLabel "Eis"@nl ;
  skos:prefLabel "Requirement"@en ;
.
nen2660-term:RequirementSeverityType
  a skos:Concept ;
  skos:broader nen2660-term:EnumerationType ;
  skos:definition "De ernst van een eis zoals gevraagd of gewenst"@nl ;
  skos:definition "The seriousness of a requirement like demanded or wished"@en ;
  skos:prefLabel "Eis ernst type"@nl ;
  skos:prefLabel "Requirement severity type"@en ;
.
nen2660-term:RequirementSourceType
  a skos:Concept ;
  skos:broader nen2660-term:EnumerationType ;
  skos:definition "Het type bron waaruit een behoefte voortkomt zoals een klant, per definitie, aanbevolen door de sector of vereist door wet/regelgeving"@nl ;
  skos:definition "The type of source from which a requirement comes like a client, by definition, recommended by the sector or demanded by law/regulation"@en ;
  skos:prefLabel "Eis bron type"@nl ;
  skos:prefLabel "Requirement source type"@en ;
.
nen2660-term:RequirementTopicType
  a skos:Concept ;
  skos:broader nen2660-term:EnumerationType ;
  skos:definition "Het entiteitsaspect waarop een eis van toepassing is"@nl ;
  skos:definition "The entity aspect a requirement applies to"@en ;
  skos:prefLabel "Eis onderwerp type"@nl ;
  skos:prefLabel "Requirement topic type"@en ;
.
nen2660-term:Solid
  a skos:Concept ;
  skos:broader nen2660-term:AggregationStateType ;
  skos:definition "Materie die kan worden opgepakt of vastgehouden, een textuur heeft en meestal stevig is. In tegenstelling tot een vloeistof, gas of plasma"@nl ;
  skos:definition "Matter that can be picked up or held, having a texture, and usually firm. Unlike a liquid, gas or plasma"@en ;
  skos:prefLabel "Solid"@en ;
  skos:prefLabel "Vaste stof"@nl ;
.
nen2660-term:SpatialRegion
  a skos:Concept ;
  skos:broader nen2660-term:PhysicalObject ;
  skos:definition "A physical object that encloses a particular area such as a room, roadway and river, that is bounded by real objects or other spatial areas (e.g., by usage or convention) and that contains primarily liquid or gaseous amount of matter"@en ;
  skos:definition "Een fysiek object dat een bepaald gebied omsluit zoals een vertrek, rijbaan en rivier, en dat wordt begrensd door reële objecten of andere ruimtelijke gebieden (bijvoorbeeld op basis van gebruik of conventie) en dat voornamelijk vloeibare of gasvormige hoeveelheid materie bevat"@nl ;
  skos:prefLabel "Ruimtelijk gebied"@nl ;
  skos:prefLabel "Spatial region"@en ;
.
nen2660-term:State
  a skos:Concept ;
  skos:broader nen2660-term:ConcreteConcept ;
  skos:definition "Temporal part of an entity during a period between two events. A state is characterized by the properties and relations of the entity"@en ;
  skos:definition "Temporeel deel van een entiteit gedurende een periode tussen twee gebeurtenissen. Een toestand wordt gekenmerkt door de eigenschappen en relaties van de entiteit"@nl ;
  skos:prefLabel "State"@en ;
  skos:prefLabel "Toestand"@nl ;
.
nen2660-term:TechnicalEntity
  a skos:Concept ;
  skos:broader nen2660-term:Entity ;
  skos:definition "An entity concerned with technical properties and relations that implements or plays functional entities"@en ;
  skos:definition "Een entiteit waarbij het gaat om technische eigenschappen en relaties die functionele entiteiten implementeert of speelt"@nl ;
  skos:prefLabel "Technical entity"@en ;
  skos:prefLabel "Technische entiteit"@nl ;
.
nen2660-term:TemporalEntity
  a skos:Concept ;
  skos:broader nen2660-term:Representation ;
  skos:definition "A temporal interval or instant"@en ;
  skos:definition "Een tijdsinterval of -moment"@nl ;
  skos:prefLabel "Temporal entity"@en ;
  skos:prefLabel "Temporele entiteit"@nl ;
.
nen2660-term:TopConcept
  a skos:Concept ;
  skos:definition "Het meest generieke concept"@nl ;
  skos:definition "The most generic concept"@en ;
  skos:prefLabel "Top concept"@en ;
  skos:prefLabel "Top concept"@nl ;
.
nen2660-term:TransferType
  a skos:Concept ;
  skos:broader nen2660-term:EnumerationType ;
  skos:definition "Het soort ding dat wordt overgedragen, hier: materiaal, informatie, energie of kracht"@nl ;
  skos:definition "The type of thing being transferred, here: material, information, energy or force"@en ;
  skos:prefLabel "Overdrachtstype"@nl ;
  skos:prefLabel "Transfer type"@en ;
.
nen2660-term:Type
  a skos:Concept ;
  skos:broader nen2660-term:AbstractConcept ;
  skos:definition "A meta-concept which instances are concepts (not individuals)"@en ;
  skos:definition "Een meta-concept waarvan instanties concepten zijn (geen individuen)"@nl ;
  skos:prefLabel "Type"@en ;
  skos:prefLabel "Type"@nl ;
.
nen2660-term:Unit
  a skos:Concept ;
  skos:definition "A particular quantity value that has been chosen as a scale for measuring other quantities the same kind"@en ;
  skos:definition "Een bepaalde hoeveelheidswaarde die is gekozen als schaal voor het meten van andere hoeveelheden van dezelfde soort"@nl ;
  skos:prefLabel "Eenheid"@nl ;
  skos:prefLabel "Unit"@en ;
.
nen2660-term:abbreviation
  a skos:Concept ;
  skos:broader skos:altLabel ;
  skos:definition "Acroniem of eerste woord als speciaal geval van een naam"@nl ;
  skos:definition "Acronym or initial word as special case of a name"@en ;
  skos:prefLabel "abbreviation"@en ;
  skos:prefLabel "afkorting"@nl ;
.
nen2660-term:aggregationStateType
  a skos:Concept ;
  skos:definition "Het hebben van een aggregatietoestandtype"@nl ;
  skos:definition "The possession of an aggregation state type"@en ;
  skos:prefLabel "aggregatietoestandtype"@nl ;
  skos:prefLabel "aggregation state type"@en ;
.
nen2660-term:begins
  a skos:Concept ;
  skos:definition "De toestand die gestart wordt door een gebeurtenis"@nl ;
  skos:definition "The state that is started by an event"@en ;
  skos:prefLabel "begins"@en ;
  skos:prefLabel "begint"@nl ;
.
nen2660-term:chemicalFormula
  a skos:Concept ;
  skos:definition "Het hebben van informatie over de chemische verhoudingen van atomen die een bepaalde chemische verbinding vormen"@nl ;
  skos:definition "The possession of information about the chemical proportions of atoms that constitute a particular chemical compound"@en ;
  skos:prefLabel "chemical formula"@en ;
  skos:prefLabel "chemische formule"@nl ;
.
nen2660-term:connectsObject
  a skos:Concept ;
  skos:definition "De fysieke objecten verbonden door een verbinding of raakvlak"@nl ;
  skos:definition "The physical objects connected by a connection or interface"@en ;
  skos:prefLabel "connects object"@en ;
  skos:prefLabel "verbindt object"@nl ;
.
nen2660-term:connectsPort
  a skos:Concept ;
  skos:definition "De poorten (als onderdeel van fysieke objecten) verbonden door een verbinding of interface"@nl ;
  skos:definition "The ports (as part of physical objects) connected by a connection or interface"@en ;
  skos:prefLabel "connects port"@en ;
  skos:prefLabel "verbindt poort"@nl ;
.
nen2660-term:consistsOf
  a skos:Concept ;
  skos:definition "De materie waarvan een reëel object of mengsel is gemaakt"@nl ;
  skos:definition "The matter a real object or mixture is made of"@en ;
  skos:prefLabel "bestaat uit"@nl ;
  skos:prefLabel "consists of"@en ;
.
nen2660-term:contains
  a skos:Concept ;
  skos:definition "De reële objecten die zich in een ruimtelijk gebied bevinden, meestal de gasvormige hoeveelheid bulkmaterie die in dat gebied aanwezig is"@nl ;
  skos:definition "The real objects located in a spatial region, typically the gaseous amount of bulk matter present in that region"@en ;
  skos:prefLabel "bevat"@nl ;
  skos:prefLabel "contains"@en ;
.
nen2660-term:ends
  a skos:Concept ;
  skos:definition "De toestand die wordt beëindigd door een gebeurtenis"@nl ;
  skos:definition "The state that is ended by an event"@en ;
  skos:prefLabel "beeindigt"@nl ;
  skos:prefLabel "ends"@en ;
.
nen2660-term:executes
  a skos:Concept ;
  skos:definition "De activiteit uitgevoerd door een fysiek object"@nl ;
  skos:definition "The activity executed by a physical object"@en ;
  skos:prefLabel "executes"@en ;
  skos:prefLabel "voert uit"@nl ;
.
nen2660-term:hasBoundary
  a skos:Concept ;
  skos:definition "De geometrische entiteit die de grens van een concreet concept vertegenwoordigt"@nl ;
  skos:definition "The geometric entity representing the boundary of a concrete concept"@en ;
  skos:prefLabel "has boundary"@en ;
  skos:prefLabel "heeft begrenzing"@nl ;
.
nen2660-term:hasFunctionalPart
  a skos:Concept ;
  skos:broader nen2660-term:hasPart ;
  skos:definition "De heeftDeel relatie van functionele aard"@nl ;
  skos:definition "The hasPart relation of a functional nature"@en ;
  skos:prefLabel "has functional part"@en ;
  skos:prefLabel "heeft functioneel deel"@nl ;
.
nen2660-term:hasInterior
  a skos:Concept ;
  skos:definition "De geometrische entiteit die het inwendige van een concreet concept vertegenwoordigt"@nl ;
  skos:definition "The geometric entity representing the interior of a concrete concept"@en ;
  skos:prefLabel "has interior"@en ;
  skos:prefLabel "heeft inwendige"@nl ;
.
nen2660-term:hasPart
  a skos:Concept ;
  skos:definition "A decomposition (hasPart) relation between concrete concepts"@en ;
  skos:definition "Een decompositie (heeftDeel) relatie tussen concrete concepten"@nl ;
  skos:prefLabel "has part"@en ;
  skos:prefLabel "heeft deel"@nl ;
.
nen2660-term:hasPartsGroup
  a skos:Concept ;
  skos:definition "Het hebben van een groep, eventueel impliciete, onderdelen"@nl ;
  skos:definition "The possession of an group of, potentially implicit, parts"@en ;
  skos:prefLabel "has parts group"@en ;
  skos:prefLabel "heeft delen groep"@nl ;
.
nen2660-term:hasQuantityKind
  a skos:Concept ;
  skos:definition "Het hebben van een grootheid"@nl ;
  skos:definition "The possession of a quantity kind"@en ;
  skos:prefLabel "has quantity kind"@en ;
  skos:prefLabel "heeft kwantiteitsoort"@nl ;
.
nen2660-term:hasRequirement
  a skos:Concept ;
  skos:definition "De (ongestructureerde) eis aan iets"@nl ;
  skos:definition "The (unstructured) requirement for something"@en ;
  skos:prefLabel "has requirement"@en ;
  skos:prefLabel "heeft eis"@nl ;
.
nen2660-term:hasSolution
  a skos:Concept ;
  skos:definition "A technical entity that is a potential solution for a functional entity"@en ;
  skos:definition "Een technische entiteit die een mogelijke oplossing is voor een functionele entiteit"@nl ;
  skos:prefLabel "has solution"@en ;
  skos:prefLabel "heeft oplossing"@nl ;
.
nen2660-term:hasState
  a skos:Concept ;
  skos:definition "De toestand van een entiteit op een bepaald tijdstip of in een bepaalde periode"@nl ;
  skos:definition "The state of an entity in a certain point or period of time"@en ;
  skos:prefLabel "has state"@en ;
  skos:prefLabel "heeft toestand"@nl ;
.
nen2660-term:hasTechnicalPart
  a skos:Concept ;
  skos:broader nen2660-term:hasPart ;
  skos:definition "A hasPart relation of a technical nature"@en ;
  skos:definition "Een heeftDeel relatie van technische aard"@nl ;
  skos:prefLabel "has technical part"@en ;
  skos:prefLabel "heeft technisch deel"@nl ;
.
nen2660-term:hasTemporalEntity
  a skos:Concept ;
  skos:definition "De abstracte temporele entiteit die een concreet concept in de tijd vertegenwoordigt"@nl ;
  skos:definition "The abstract temporal entity representing a concrete concept in time"@en ;
  skos:prefLabel "has temporal entity"@en ;
  skos:prefLabel "heeft temporele entiteit"@nl ;
.
nen2660-term:hasUnit
  a skos:Concept ;
  skos:definition "Het hebben van een eenheid"@nl ;
  skos:definition "The possession of a unit"@en ;
  skos:prefLabel "has unit"@en ;
  skos:prefLabel "heeft eenheid"@nl ;
.
nen2660-term:isBoundBy
  a skos:Concept ;
  skos:definition "Het fysieke object dat een ruimtelijk gebied begrensd"@nl ;
  skos:definition "The physical object that bounds a spatial region"@en ;
  skos:prefLabel "is begrensd door"@nl ;
  skos:prefLabel "is bound by"@en ;
.
nen2660-term:isConnectedTo
  a skos:Concept ;
  skos:definition "De topologische relatie tussen fysieke objecten"@nl ;
  skos:definition "The topological relation between physical objects"@en ;
  skos:prefLabel "is connected to"@en ;
  skos:prefLabel "is verbonden met"@nl ;
.
nen2660-term:isDescribedBy
  a skos:Concept ;
  skos:definition "Het informatie object dat iets beschrijft"@nl ;
  skos:definition "The information object that describes something"@en ;
  skos:prefLabel "is beschreven door"@nl ;
  skos:prefLabel "is described by"@en ;
.
nen2660-term:isImplementedBy
  a skos:Concept ;
  skos:broader nen2660-term:hasSolution ;
  skos:definition "De technische entiteit die een functionele entiteit implementeert"@nl ;
  skos:definition "The technical entity that implements a functional entity"@en ;
  skos:prefLabel "is geimplementeerd door"@nl ;
  skos:prefLabel "is implemented by"@en ;
.
nen2660-term:isPlanFor
  a skos:Concept ;
  skos:definition "A potentially realized entity according to this planned entity"@en ;
  skos:definition "Een potentieel gerealiseerde entiteit volgens deze geplande entiteit"@nl ;
  skos:prefLabel "is plan for"@en ;
  skos:prefLabel "is plan voor"@nl ;
.
nen2660-term:isRealizedBy
  a skos:Concept ;
  skos:broader nen2660-term:isPlanFor ;
  skos:definition "De gerealiseerde entiteit die een geplande entiteit realiseert"@nl ;
  skos:definition "The realized entity that realizes a planned entity"@en ;
  skos:prefLabel "is gerealiseerd door"@nl ;
  skos:prefLabel "is realized by"@en ;
.
nen2660-term:overConnection
  a skos:Concept ;
  skos:definition "De verbinding waarover een interactie tussen fysieke objecten plaatsvindt"@nl ;
  skos:definition "The connection over which an interaction between physical objects takes place"@en ;
  skos:prefLabel "over connection"@en ;
  skos:prefLabel "over verbinding"@nl ;
.
nen2660-term:overInterface
  a skos:Concept ;
  skos:definition "Het raakvlak waarover een interactie tussen fysieke objecten plaatsvindt"@nl ;
  skos:definition "The interface over which an interaction between physical objects takes place"@en ;
  skos:prefLabel "over interface"@en ;
  skos:prefLabel "over raakvlak"@nl ;
.
nen2660-term:participatesIn
  a skos:Concept ;
  skos:definition "De interactie waaraan een fysiek object deelneemt"@nl ;
  skos:definition "The interaction a physical object participates in"@en ;
  skos:prefLabel "participates in"@en ;
  skos:prefLabel "participeert in"@nl ;
.
nen2660-term:portion
  a skos:Concept ;
  skos:definition "Het relatieve deel van een materiedeel"@nl ;
  skos:definition "The relative portion of a matter portion"@en ;
  skos:prefLabel "aandeel"@nl ;
  skos:prefLabel "portion"@en ;
.
nen2660-term:requirementSeverityType
  a skos:Concept ;
  skos:definition "Het hebben van een ernsttype door een eis"@nl ;
  skos:definition "The possession of a severity type by a requirement"@en ;
  skos:prefLabel "eis ernst type"@nl ;
  skos:prefLabel "requirement severity type"@en ;
.
nen2660-term:requirementSourceType
  a skos:Concept ;
  skos:definition "Het hebben van een brontype door een eis"@nl ;
  skos:definition "The possession of a source type by a requirement"@en ;
  skos:prefLabel "eis bron type"@nl ;
  skos:prefLabel "requirement source type"@en ;
.
nen2660-term:requirementTopicType
  a skos:Concept ;
  skos:definition "Het hebben van een onderwerptype door een eis"@nl ;
  skos:definition "The possession of a topic type by a requirement"@en ;
  skos:prefLabel "eis onderwerp type"@nl ;
  skos:prefLabel "requirement topic type"@en ;
.
nen2660-term:transferType
  a skos:Concept ;
  skos:definition "Het hebben van een overdrachtstype door een interactie"@nl ;
  skos:definition "The possession of a transfer type by an interaction"@en ;
  skos:prefLabel "overdrachtstype"@nl ;
  skos:prefLabel "transfer type"@en ;
.
nen2660-term:transforms
  a skos:Concept ;
  skos:definition "Het object getransformeerd door een activiteit"@nl ;
  skos:definition "The object transformed by an activity"@en ;
  skos:prefLabel "transformeert"@nl ;
  skos:prefLabel "transforms"@en ;
.
nen2660-term:triggers
  a skos:Concept ;
  skos:definition "De gebeurtenis getriggerd door een entiteit"@nl ;
  skos:definition "The event triggert by an entity"@en ;
  skos:prefLabel "triggers"@en ;
  skos:prefLabel "triggert"@nl ;
.